src/tls/HandshakeLog.Common.fst
@@ -1,0 +1,40 @@
+module HandshakeLog.Common
+
+open FStar.Integers
+open FStar.HyperStack.ST
+
+module G = FStar.Ghost
+module List = FStar.List.Tot
+
+module HS = FStar.HyperStack
+module B = LowStar.Buffer
+
+module C = TLSConstants
+module Hash = Hashing
+module HashSpec = Hashing.Spec
+module HSM = HandshakeMessages
+
+module LP = LowParse.Low.Base
+
+type hbytes = Spec.Hash.Definitions.bytes
+
+
+/// TODO: LowParse definition of saying buf is a valid serialization of m
+
+assume
+val valid_parsing_aux (m:HSM.hs_msg) (buf:B.buffer uint_8) (h:HS.mem) : Type0
+
+
+/// Helper to enforce spatial safety of indices in the st input buffer
+/// and that the buffer is a serialization of m
+
+let valid_parsing (m:HSM.hs_msg) (from to:uint_32) (b:B.buffer uint_8) (h:HS.mem) =
+  from <= to /\
+  to <= B.len b /\
+  (let buf = B.gsub b from (to - from) in
+   valid_parsing_aux m buf h)
+
+
+/// TODO: define using high-level serializers from LowParse
+
+val format_hs_msg (m:HSM.hs_msg) : Tot hbytes
